done

Others/Aha.v
@@ -12,15 +12,15 @@ Inductive Term :=
 | iszero    (t : Term)
 | cond      (p : Term) (t1 : Term) (t2 : Term).
 
-Fixpoint isnv (t: Term) : bool :=
-    match t with
+Fixpoint isnv (tm: Term) : bool :=
+    match tm with
     | zero      => true
-    | succ t'   => isnv t'
+    | succ tm'  => isnv tm'
     | _         => false
     end.
 
-Fixpoint reduce (t : Term) : option Term :=
-    match t with
+Fixpoint reduce (tm : Term) : option Term :=
+    match tm with
     | cond t t1 _       => Some t1
     | cond f _  t2      => Some t2
     | cond k t1 t2      => option_map (fun z => cond z t1 t2) (reduce k)
@@ -34,24 +34,24 @@ Fixpoint reduce (t : Term) : option Term :=
     | _                 => None
     end.
 
-Fixpoint depth (t : Term) : nat :=
-    match t with
+(* size *)
+Fixpoint depth (tm : Term) : nat :=
+    match tm with
     | zero | t | f  => 1
     | succ n        => 1 + depth n
     | iszero n      => 1 + depth n
     | pred n        => 1 + depth n
-    | cond p t1 t2  => 1 + (max (depth p) (max (depth t1) (depth t2)))
+    | cond p t1 t2  => 1 + (depth p) + (depth t1) + (depth t2)
     end.
 
 (* too obvious *)
 Lemma le_S : forall (a b : nat), a < b -> S a < S b. Proof. intros. lia. Qed.
 Lemma le_O : forall (a : nat), 0 < S a. Proof. intros. lia. Qed.
 
-(* the measure might be wrong *)
-Function eval (t : Term) {measure depth t} : Term :=
-    match reduce t with
-    | None      => t
-    | Some t'   => eval t'
+Function eval (tm : Term) {measure depth tm} : Term :=
+    match reduce tm with
+    | None      => tm
+    | Some tm'  => eval tm'
     end.
 Proof.
     intro tm. induction tm; 
@@ -117,8 +117,41 @@ Proof.
             simpl in H. apply H.
         }
       + destruct tm; inversion H0.
-        
-
-Abort.
+        { simpl. lia. }
+        { 
+            destruct (isnv tm); inversion H0.
+            simpl. lia.
+        }
+    - destruct (reduce tm1) eqn: T.
+      + destruct tm1.
+        * simpl. inversion H0. lia.
+        * simpl. inversion H0. lia.
+        * inversion teq.
+        * simpl in H0. inversion H0.
+          simpl. apply le_S.
+          assert (depth t0 < depth (succ tm1)).
+          apply IHtm1. reflexivity.
+        simpl in H. lia.
+        * simpl in H0. inversion H0.
+          simpl. apply le_S.
+          assert (depth t0 < depth (pred tm1)).
+          apply IHtm1. reflexivity.
+          simpl in H. lia.
+        * simpl in H0. inversion H0.
+          simpl. apply le_S.
+          assert (depth t0 < depth (iszero tm1)).
+          apply IHtm1. reflexivity.
+          simpl in H. lia.
+        * simpl in H0. inversion H0. simpl. apply le_S.
+          assert (depth t0 < depth (cond tm1_1 tm1_2 tm1_3)).
+          apply IHtm1. reflexivity. 
+          simpl in H. lia.
+      + destruct tm1; inversion H0.
+        * simpl. lia.
+        * simpl. lia.
+Defined.
 
 Compute (reduce (iszero zero)).
+
+Definition t1 := cond (cond (iszero zero) f t) (succ zero) (succ (succ zero)).
+Compute (eval t1).
